@prefix : <https://schema.org/> .
@prefix todo: <https://todo/> .
@prefix rdf: <http://www.w3.org/1999/02/22-rdf-syntax-ns#> .
@prefix rdfs: <http://www.w3.org/2000/01/rdf-schema#> .

#
# This file contains information about Thing > Intangible > AnimalPolicy.
#
# @see https://github.com/schemaorg/suggestions-questions-brainstorming/issues/39
#

#
# Classes
#
:AnimalPolicy a rdfs:Class ;
    rdfs:subClassOf :Intangible;
    rdfs:label "AnimalPolicy" ;
    rdfs:comment """
        Provides information about how the operators of an [[Organization]], [[Place]] or [[Service]] deal with
        people accompanied by animals. This is relevant for people who need an assistance animal
        (e.g. a guide dog), or travel with a pet.
    """ .

#
# Properties
#
:allowsAnyDogs a rdf:Property ;
    :domainIncludes :AnimalPolicy ;
    :rangeIncludes :Boolean ;
    rdfs:label "allowsAnyDogs" ;
    rdfs:comment """
        True if the place allows visitors to bring dogs in general, False if bringing them is explicitly
        prohibited (with exception of assistance dogs, if allowsAssistanceDogs is True).
    """ .

:allowsAssistanceDogs a rdf:Property ;
    :domainIncludes :AnimalPolicy ;
    :rangeIncludes :Boolean ;
    rdfs:label "allowsAssistanceDogs" ;
    rdfs:comment """
        True if the place allows visitors to bring assistance/guide dogs, False if bringing them is
        explicitly prohibited.
    """ .

:allowsDogsOnlyWithMuzzle	a rdf:Property ;
    :domainIncludes :AnimalPolicy ;
    :rangeIncludes :Boolean ;
    rdfs:label "allowsDogsOnlyWithMuzzle" ;
    rdfs:comment """
        True if the place denies entry to visitors bringing a dogs without muzzles,
        False if dogs without muzzles are explicitly allowed.
    """ .

:suppliesWaterForAnimals a rdf:Property ;
    :domainIncludes :AnimalPolicy ;
    :rangeIncludes :Boolean ;
    rdfs:label "suppliesWaterForAnimals" ;
    rdfs:comment """
        True if the place supplies water for accompanying animals, False if explicitly not.
    """ .

:allowsDogsOnlyWithLeash	a rdf:Property ;
    :domainIncludes :AnimalPolicy ;
    :rangeIncludes :Boolean ;
    rdfs:label "allowsDogsOnlyWithLeash" ;
    rdfs:comment """
        True if the place denies entry to visitors bringing a dogs without leash,
        False if dogs without leash are explicitly allowed.
    """ .