@prefix : <https://schema.org/> .
@prefix todo: <https://todo/> .
@prefix rdf: <http://www.w3.org/1999/02/22-rdf-syntax-ns#> .
@prefix rdfs: <http://www.w3.org/2000/01/rdf-schema#> .

#
# This file contains information about Thing > Product > Vehicle > Elevator.
#
# @see https://github.com/schemaorg/suggestions-questions-brainstorming/issues/39
#

#
# Classes
#
:Elevator a rdfs:Class ;
    rdfs:subClassOf :Vehicle;
    rdfs:label "Elevator" ;
    :sameAs <https://dbpedia.org/page/Elevator> ;
    :sameAs <https://www.wikidata.org/wiki/Q132911> ;
    rdfs:comment """
        Describes a physical elevator that transports people or goods vertically. If properties of the supertypeVehicle are used, they should describe the
        elevator’s cabin, moving platform, or sling. If a cabin or platform is part of the elevator, it's width and depth properties should be included for
        saccessibility.
    """ .

#
# Properties
#
:door a rdf:Property ;
    :domainIncludes :Elevator ;
    :rangeIncludes :Door ;
    rdfs:label "door" ;
    rdfs:comment """
        List containing descriptions of the elevator’s door(s).
    """ .

:hasDoorsInOppositeDirections a rdf:Property ;
    :domainIncludes :Elevator ;
    :rangeIncludes :Boolean ;
    rdfs:label "hasDoorsInOppositeDirections" ;
    rdfs:comment """
        True if the equipment has doors in opposite directions. Relevant for people using a wheelchair, rollator,
        cargo bike or pushchair to know if they have to turn.
    """ .

:connectedFloorLevels a rdf:Property ;
    :domainIncludes :Elevator ;
    :rangeIncludes :Text ;
    rdfs:label "connectedFloorLevels" ;
    rdfs:comment """
        The connected floor levels in a multi-storey building, as list, if applicable. Since counting systems
        vary internationally, the local system should be used where possible.
    """ .

:operationalStatus a rdf:Property ;
    :domainIncludes :Elevator ;
    :rangeIncludes :OperationalStatus ;
    rdfs:label "operationalStatus" ;
    rdfs:comment """
        Describes current usability of the facility. Can be used for real-time status updates.
    """ .

:alternativeWays a rdf:Property ;
    :domainIncludes :Elevator ;
    :rangeIncludes :Thing ;
    rdfs:label "alternativeWays" ;
    rdfs:comment """
        If there are alternative routes to this elevator, they can be linked using this property.
    """ .

