@prefix : <https://schema.org/> .
@prefix todo: <https://todo/> .
@prefix rdf: <http://www.w3.org/1999/02/22-rdf-syntax-ns#> .
@prefix rdfs: <http://www.w3.org/2000/01/rdf-schema#> .

#
# This file contains information about Thing > Product > Vehicle > Escalator.
#
# @see https://github.com/schemaorg/suggestions-questions-brainstorming/issues/39
#

#
# Classes
#
:Escalator a rdfs:Class ;
    rdfs:subClassOf :Vehicle;
    rdfs:label "Escalator" ;
    :sameAs <https://dbpedia.org/page/Escalator> ;
    :sameAs <https://www.wikidata.org/wiki/Q15003> ;
    rdfs:comment """
        An escalator is a moving staircase which carries people between floors of a building or structure.
        It consists of a motor-driven chain of individually linked steps on a track which cycle on a pair of
        tracks which keep them horizontal.
    """ .

:Stairlift a rdfs:Class ;
    rdfs:subClassOf :Elevator;
    rdfs:label "Stairlift" ;
    :sameAs <https://dbpedia.org/page/Stairlift> ;
    :sameAs <https://www.wikidata.org/wiki/Q1894866> ;
    rdfs:comment """
        A stair lift is a mechanical device for lifting people up and down stairs. For sufficiently wide
        stairs, a rail is mounted to the treads of the stairs. A chair or lifting platform is attached to
        the rail. A person gets onto the chair or platform and is lifted up or down the stairs by the chair
        which moves along the rail.
    """ .

#
# Properties
#
:connectedFloorLevels a rdf:Property ;
    :domainIncludes :Escalator ;
    :rangeIncludes :Text ;
    rdfs:label "connectedFloorLevels" ;
    rdfs:comment """
        The connected floor levels in a multi-storey building, as list, if applicable. Since counting systems
        vary internationally, the local system should be used where possible.
    """ .

:stairs a rdf:Property ;
    :domainIncludes :Escalator ;
    :rangeIncludes :Stairs ;
    rdfs:label "stairs" ;
    rdfs:comment """
        Describes the escalator’s staircase. Relevant for passengers if an escalator is out of service, and
        there is no alternative route.
    """ .

:handrails a rdf:Property ;
    :domainIncludes :Escalator ;
    :rangeIncludes :Handrails ;
    rdfs:label "handrails" ;
    rdfs:comment """
        Provides information about the escalator’s handrails.
    """ .

:operationalStatus a rdf:Property ;
    :domainIncludes :Escalator ;
    :rangeIncludes :OperationalStatus	 ;
    rdfs:label "operationalStatus" ;
    rdfs:comment """
        Describes current usability of the escalator. Can be used for real-time status updates.
    """ .

