@prefix : <https://schema.org/> .
@prefix todo: <https://todo/> .
@prefix rdf: <http://www.w3.org/1999/02/22-rdf-syntax-ns#> .
@prefix rdfs: <http://www.w3.org/2000/01/rdf-schema#> .

#
# This file contains information about Thing > Product > GrabBar.
#
# @see https://github.com/schemaorg/suggestions-questions-brainstorming/issues/39
#

#
# Classes
#
:GrabBar a rdfs:Class ;
    rdfs:subClassOf :Product;
    rdfs:label "GrabBar" ;
    rdfs:comment """
        Grab bars are safety devices designed to enable a person to maintain balance, lessen fatigue while
        standing, hold some of their weight while maneuvering, or have something to grab onto in case of a
        slip or fall. A caregiver may use a grab bar to assist with transferring a patient from one place to
        another. A worker may use a grab bar to hold on to as he or she climbs, or in case of a fall.
    """ .

#
# Properties
#
:isOnUsersLeftSide a rdf:Property ;
    :domainIncludes :GrabBar ;
    :rangeIncludes :Boolean ;
    rdfs:label "isOnUsersLeftSide" ;
    rdfs:comment """
        True if there is a grab bar on left side(from the perspective of somebody using the toilet),
        false if not, undefined if condition is unknown.
    """ .

:isOnUsersRightSide a rdf:Property ;
    :domainIncludes :GrabBar ;
    :rangeIncludes :Boolean ;
    rdfs:label "isOnUsersRightSide" ;
    rdfs:comment """
        True if there is a grab bar on right side(from the perspective of somebody using the toilet),
        false if not, undefined if condition is unknown.
    """ .

:heightFromFloor a rdf:Property ;
    :domainIncludes :GrabBar ;
    :rangeIncludes :QuantitativeValue ;
    rdfs:label "heightFromFloor" ;
    rdfs:comment """
        Indicates the grab bar height at the position where they are meant to be held,
        measured as distance from the floor.
    """ .

:isFoldable a rdf:Property ;
    :domainIncludes :GrabBar ;
    :rangeIncludes :Boolean ;
    rdfs:label "isFoldable" ;
    rdfs:comment """
        True if it is foldable, False if it is fixed (not foldable)
    """ .

