@prefix : <https://schema.org/> .
@prefix todo: <https://todo/> .
@prefix rdf: <http://www.w3.org/1999/02/22-rdf-syntax-ns#> .
@prefix rdfs: <http://www.w3.org/2000/01/rdf-schema#> .

#
# This file contains information about Thing > GroundSurface.
#
# @see https://github.com/schemaorg/suggestions-questions-brainstorming/issues/39
#

#
# Classes
#
:GroundSurfaceEnumeration a rdfs:Class ;
    rdfs:subClassOf :Enumeration ;
    rdfs:label "GroundSurfaceEnumeration" ;
    :sameAs <http://live.dbpedia.org/page/Surface> ;
    :sameAs <https://wiki.openstreetmap.org/wiki/Key:surface> ;
    rdfs:comment """
        Describes the quality of a physical ground surface.
        Use this to describe road or sidewalk conditions, or to provide indoor accessibility information.
    """ .

:GroundSurfacePaved a :GroundSurfaceEnumeration ;
    rdfs:label "GroundSurfacePaved" ;
    rdfs:comment """
        A feature that is predominantly paved; i.e., it is covered with paving stones, concrete or bitumen.
        This value gives only a rough description; use a more precise value if possible.
    """ .

:GroundSurfaceAsphalt a :GroundSurfaceEnumeration ;
    rdfs:label "GroundSurfaceAsphalt" ;
    :sameAs <http://live.dbpedia.org/page/Asphalt> ;
    :sameAs <https://wiki.openstreetmap.org/wiki/Tag:surface%3Dasphalt> ;
    rdfs:comment """
       Short for asphalt concrete - mineral aggregate bound by asphalt. Most such features are tagged as
       paved without specifying exact surface.
    """ .

:GroundSurfaceConcrete a :GroundSurfaceEnumeration ;
    rdfs:label "GroundSurfaceConcrete" ;
    :sameAs <https://dbpedia.org/page/Concrete> ;
    :sameAs <https://www.wikidata.org/wiki/Q22657> ;
    rdfs:comment """
        Cement based concrete, forming a large surface, typically cast in place and may have predetermined
        breaking joints. For pre-fabricated plates, please use concrete:plates or concrete:lanes if you know
        how the concrete is laid out and one of these tags fits.
    """ .

:GroundSurfaceConcreteLanes a :GroundSurfaceEnumeration ;
    rdfs:label "GroundSurfaceConcreteLanes" ;
    :sameAs <https://dbpedia.org/page/Lane> ;
    :sameAs <https://wiki.openstreetmap.org/wiki/Tag:surface%3Dconcrete:lanes> ;
    rdfs:comment """
        Long, narrow concrete elements for a two-tracked vehicle (motorcars) so that the tires always hit the
        concrete. There might be sand, ground, grass, pavers, asphalt, etc. in between them. Note that if you tag
        a single-tracked way you just use concrete, since there are no lanes.
    """ .

:GroundSurfaceConcretePlates a :GroundSurfaceEnumeration ;
    rdfs:label "GroundSurfaceConcretePlates" ;
    :sameAs <https://wiki.openstreetmap.org/wiki/Tag:surface%3Dconcrete:plates> ;
    rdfs:comment """
        Heavy duty plates chained closely together on the short side. Might have tar or sand in between the connections.
    """ .

:GroundSurfacePavingStones a :GroundSurfaceEnumeration ;
    rdfs:label "GroundSurfacePavingStones" ;
    :sameAs <https://wiki.openstreetmap.org/wiki/Tag:surface%3Dpaving_stones> ;
    rdfs:comment """
        A relatively smooth surface paved with artificial blocks (block pavers, bricks) or natural stones
        (flagstones), with a flat top. The gaps between individual paving stones are very narrow, either
        because the stones have a perfectly regular shape (rectangular, or any surface-filling shape) or
        because they have been carefully selected, fitted and placed in order to form an even, closed surface.
    """ .

:GroundSurfaceSett a :GroundSurfaceEnumeration ;
    rdfs:label "GroundSurfaceSett" ;
    :sameAs <https://wiki.openstreetmap.org/wiki/Tag:surface%3Dsett> ;
    rdfs:comment """
        Sett paving, formed from natural stones cut to a regular shape. The stones do not cover the surface
        completely, unlike paving_stones.
    """ .

:GroundSurfaceUnhewnCobblestone a :GroundSurfaceEnumeration ;
    rdfs:label "GroundSurfaceUnhewnCobblestone" ;
    :sameAs <https://wiki.openstreetmap.org/wiki/Tag:surface%3Dunhewn_cobblestone> ;
    rdfs:comment """
        Raw cobblestone of natural, uncut, rounded stones. Unlike pebblestone firmly connected to the ground.
    """ .

:GroundSurfaceCobblestone a :GroundSurfaceEnumeration ;
    rdfs:label "GroundSurfaceCobblestone" ;
    :sameAs <https://wiki.openstreetmap.org/wiki/Tag:surface%3Dcobblestone> ;
    rdfs:comment """
        Generic value for cobblestone in the colloquial sense. It's better to use a more precise value
        such as sett or unhewn_cobblestone
    """ .

:GroundSurfaceMetal a :GroundSurfaceEnumeration ;
    rdfs:label "GroundSurfaceMetal" ;
    rdfs:comment """
        Used for metal surfaced bridges, or for temporary tracks over fields for normal road vehicles
        or site traffic.
    """ .

:GroundSurfaceWood a :GroundSurfaceEnumeration ;
    rdfs:label "GroundSurfaceWood" ;
    :sameAs <https://wiki.openstreetmap.org/wiki/Tag:surface%3Dwood> ;
    rdfs:comment """
        Used for wood surfaced bridges, plank walkways, and garden decking
    """ .

:GroundSurfaceSteppingStones a :GroundSurfaceEnumeration ;
    rdfs:label "GroundSurfaceSteppingStones" ;
    :sameAs <https://www.wikidata.org/wiki/Q1415899> ;
    rdfs:comment """
        Stones or plates individually arranged in a row, allowing to walk on, surrounded by an unpaved
        medium such as grass or water
    """ .

:GroundSurfaceUnpaved a :GroundSurfaceEnumeration ;
    rdfs:label "GroundSurfaceUnpaved" ;
    :sameAs <https://wiki.openstreetmap.org/wiki/Tag:surface%3Dunpaved> ;
    rdfs:comment """
        A feature that is predominantly unsealed (unpaved); i.e., it has a loose covering ranging from
        compacted stone chippings to earth. Unpaved roads may, in aerial imagery, show evidence of water
        along their course; in such circumstances, the waterway should not be tagged as a stream, though
        it might appear as such. This value gives only a rough description; use a more precise value if
        possible.
    """ .

:GroundSurfaceCompacted a :GroundSurfaceEnumeration ;
    rdfs:label "GroundSurfaceCompacted" ;
    :sameAs <https://wiki.openstreetmap.org/wiki/Tag:surface%3Dcompacted> ;
    rdfs:comment """
        A mixture of larger (e.g., gravel) and smaller (e.g., sand) parts, compacted (e.g., with a roller),
        so the surface is more stable than loose gravel. Used, for example, for park paths, better tracks,
        some service ways, â€¦ Best sort of ways below paving with asphalt, concrete, paving stones. Sometimes
        known as water-bound macadam. Mixture and compacting leads to more grip and stability.
    """ .

:GroundSurfaceFineGravel a :GroundSurfaceEnumeration ;
    rdfs:label "GroundSurfaceFineGravel" ;
    rdfs:comment """
        A multilayer pavement with a stone or gravel basis and a topmost surface of firm, granular grit,
        basalt or quartz, as invented by the Roman empire. Easy to walk, jog, cycle or ride on. In hilly
        areas mostly with drainage channels and concave cross-section for proper water shedding. Motorized
        vehicles will not move stones if the way is maintained properly, and bicycles tires will not leave
        any imprints at least in dry weather. If the topmost surface is eroded or loose gravel aggravate
        please use gravel instead.
    """ .

:GroundSurfaceGravel a :GroundSurfaceEnumeration ;
    rdfs:label "GroundSurfaceGravel" ;
    :sameAs <https://dbpedia.org/page/Gravel> ;
    :sameAs <https://www.wikidata.org/wiki/Q133833> ;
    rdfs:comment """
        Broken/crushed rock with sharp edges, known as ballast on railways. Usually loosely arranged. Typical
        size for road and surface construction range between 4 and 8 cm. Gravel can be used as a ground-layer
        for compacted.
    """ .

:GroundSurfaceRock a :GroundSurfaceEnumeration ;
    rdfs:label "GroundSurfaceRock" ;
    :sameAs <https://wiki.openstreetmap.org/wiki/Tag:surface%3Drock> ;
    rdfs:comment """
        Exposed rock or big pieces of rock used to improve path quality. Typically in mountainous areas.
    """ .

:GroundSurfacePebblestone a :GroundSurfaceEnumeration ;
    rdfs:label "GroundSurfacePebblestone" ;
    rdfs:comment """
        Pebbles are stones rounded by waves or river flow. Typical size range from 2 to 8 cm. Describing a
        surface in OSM they are loosely arranged. Like gravel pebbles can be used as a building part of compacted.
    """ .

:GroundSurfaceGround a :GroundSurfaceEnumeration ;
    rdfs:label "GroundSurfaceGround" ;
    rdfs:comment """
        No special surface, the ground itself has marks of human or animal usage. This value gives only a rough
        description; if possible, use a more precise value such as grass, clay, sand, earth, gravel or pebblestone.
    """ .

:GroundSurfaceDirt a :GroundSurfaceEnumeration ;
    rdfs:label "GroundSurfaceDirt" ;
    :sameAs <http://live.dbpedia.org/page/Dirt> ;
    :sameAs <https://wiki.openstreetmap.org/wiki/Tag:surface%3Ddirt> ;
    rdfs:comment """
        Probably very similar to ground. Like all this, it is prone to erosion and therefore often uneven.
        Gravel is sometimes mistakenly called dirt. Some compacted surfaces are sometimes called 'dirt' too,
        please consider the definition of compacted.
    """ .

:GroundSurfaceEarth a :GroundSurfaceEnumeration ;
    rdfs:label "GroundSurfaceEarth" ;
    :sameAs <https://www.wikidata.org/wiki/Q2488752> ;
    rdfs:comment """
        Probably a type of ground. Usually natural, but may also apply to artificial preparations of soil.
        Duplicate of dirt.
    """ .

:GroundSurfaceGrass a :GroundSurfaceEnumeration ;
    rdfs:label "GroundSurfaceGrass" ;
    :sameAs <https://www.wikidata.org/wiki/Q643352> ;
    rdfs:comment """
        Grass covered ground. Mostly nice to walk. May turn into surface=dirt or become overgrown and disappear.
    """ .

:GroundSurfaceGrassPaver a :GroundSurfaceEnumeration ;
    rdfs:label "GroundSurfaceGrassPaver" ;
    :sameAs <https://wiki.openstreetmap.org/wiki/Tag:surface%3Dgrass_paver> ;
    rdfs:comment """
        A sort of permeable paving using regular cell structure, where the voids in this structure enable
        rainwater to drain into the ground and the structure itself increases the load bearing capability.
        Often used for parking lots or infrequent used ways like for emergency-vehicles.
    """ .

:GroundSurfaceMud a :GroundSurfaceEnumeration ;
    rdfs:label "GroundSurfaceMud" ;
    :sameAs <https://wiki.openstreetmap.org/wiki/Tag:surface%3Dmud> ;
    rdfs:comment """
        Similar to ground but most of the year wet which gives a soft ground with low carrying capacity.
        Mostly found on wetland like swamps or in tidal areas. Sometimes also found on slopes draining onto a way.
    """ .

:GroundSurfaceSand a :GroundSurfaceEnumeration ;
    rdfs:label "GroundSurfaceSand" ;
    :sameAs <https://dbpedia.org/page/Sand> ;
    :sameAs <https://www.wikidata.org/wiki/Q34679> ;
    rdfs:comment """
        Small to very small fractions (less than 2mm) of rock.
    """ .

:GroundSurfaceWoodchips a :GroundSurfaceEnumeration ;
    rdfs:label "GroundSurfaceWoodchips" ;
    :sameAs <https://www.wikidata.org/wiki/Q663690> ;
    rdfs:comment """
        Woodchips as a surface
    """ .

:GroundSurfaceSnow a :GroundSurfaceEnumeration ;
    rdfs:label "GroundSurfaceSnow" ;
    :sameAs <https://dbpedia.org/page/Snow> ;
    :sameAs <https://www.wikidata.org/wiki/Q7561> ;
    rdfs:comment """
        Winter roads surfaced with compacted snow.
    """ .

:GroundSurfaceIce a :GroundSurfaceEnumeration ;
    rdfs:label "GroundSurfaceIce" ;
    :sameAs <https://dbpedia.org/page/Ice> ;
    :sameAs <https://www.wikidata.org/wiki/Q23392> ;
    rdfs:comment """
        Ice roads, winter roads
    """ .

:GroundSurfaceSalt a :GroundSurfaceEnumeration ;
    rdfs:label "GroundSurfaceSalt" ;
    :sameAs <https://www.wikidata.org/wiki/Q12370> ;
    rdfs:comment """
        Dry salt lakes
    """ .

:GroundSurfaceClay a :GroundSurfaceEnumeration ;
    rdfs:label "GroundSurfaceClay" ;
    :sameAs <https://dbpedia.org/page/Clay> ;
    :sameAs <https://www.wikidata.org/wiki/Q42302> ;
    rdfs:comment """
        Most common on tennis courts. Sometimes used for other sports: soccer, athletic tracks, boules, etc.
    """ .

:GroundSurfaceTartan a :GroundSurfaceEnumeration ;
    rdfs:label "GroundSurfaceTartan" ;
    :sameAs <https://wiki.openstreetmap.org/wiki/Tag:surface%3Dtartan> ;
    rdfs:comment """
        A synthetic, all-weather surface typically used in running and other sport tracks. Although Tartan
        is a trademark, it is used as a generic term due to its widespread usage.
    """ .

:GroundSurfaceArtificialTurf a :GroundSurfaceEnumeration ;
    rdfs:label "GroundSurfaceArtificialTurf" ;
    :sameAs <https://wiki.openstreetmap.org/wiki/Tag:surface%3Dartificial_turf> ;
    rdfs:comment """
        An all-weather surface made from synthetic fibres to look and feel like natural grass. Often used
        for tracks and pitches of sports such as football, baseball, etc.
    """ .

:GroundSurfaceAcrylic a :GroundSurfaceEnumeration ;
    rdfs:label "GroundSurfaceAcrylic" ;
    :sameAs <https://dbpedia.org/page/Acrylic_resin> ;
    :sameAs <https://wiki.openstreetmap.org/wiki/Tag:surface%3Dacrylic> ;
    rdfs:comment """
        An artificial surface covered with acrylic resin-bound coating. Often used for tennis courts,
        basketball courts, etc. Prominent brands include: DecoTurf, GreenSet and so on.
    """ .

:GroundSurfaceMetalGrid a :GroundSurfaceEnumeration ;
    rdfs:label "GroundSurfaceMetalGrid" ;
    :sameAs <https://www.wikidata.org/wiki/Q58328221> ;
    rdfs:comment """
        Metal grids are often used as a surface on industrial-style bridges or stairs. When wet, the surface
        can become very slippery, especially for bikes. The surface can also be unsuitable for dogs, due to
        the sharp edges and the look-through effect.
    """ .

:GroundSurfaceCarpet a :GroundSurfaceEnumeration ;
    rdfs:label "GroundSurfaceCarpet" ;
    :sameAs <https://dbpedia.org/page/Carpet> ;
    :sameAs <https://www.wikidata.org/wiki/Q29167278> ;
    rdfs:comment """
        Carpet may be used for some sport courts such as indoor tennis courts.
    """ .

#
# Properties
#
:isEven a rdf:Property ;
    :domainIncludes :GroundSurface ;
    :rangeIncludes :Boolean ;
    rdfs:label "isEven" ;
    rdfs:comment """
        True if the surface is even and not plastered, False if not even or plastered.
    """ .

:isLevel a rdf:Property ;
    :domainIncludes :GroundSurface ;
    :rangeIncludes :Boolean ;
    rdfs:label "isLevel" ;
    rdfs:comment """
        True if the described object can be used step-free and the ground/floor is level, False if not
        (e.g. if users have to take a step to use the main functionality). Can be True even if the
        ground/floor is not perfectly even but plastered, for example - for this case, you can provide a
        surface property instead.
    """ .

:surface a rdf:Property ;
    :domainIncludes :GroundSurface ;
    :rangeIncludes :Text ;
    rdfs:label "surface" ;
    rdfs:comment """
        Rating of surface/sidewalk conditions. Use strings from
        https://wiki.openstreetmap.org/wiki/Key:surface as values, for example.
    """ .

:slopeAngle a rdf:Property ;
    :domainIncludes :GroundSurface ;
    :rangeIncludes :QuantitativeValue ;
    rdfs:label "slopeAngle" ;
    rdfs:comment """
        Angle of the slope that this ground surface has, if applicable.

    """ .

