@prefix : <https://schema.org/> .
@prefix todo: <https://todo/> .
@prefix rdf: <http://www.w3.org/1999/02/22-rdf-syntax-ns#> .
@prefix rdfs: <http://www.w3.org/2000/01/rdf-schema#> .

#
# This file contains information about Thing > Intangible > Service > MobilityService.
#
# @see https://github.com/schemaorg/suggestions-questions-brainstorming/issues/39
#

#
# Classes
#
:MobilityService a rdfs:Class ;
    rdfs:subClassOf :Service;
    rdfs:label "MobilityService" ;
    rdfs:comment """
        An aggregation of references to services that are usually associated with mobility in public transport.
        This is relevant as accessibility information for travellers.
    """ .

#
# Properties
#
:serviceOperator a rdf:Property ;
    :domainIncludes :MobilityService ;
    :rangeIncludes :Organization ;
    rdfs:label "serviceOperator" ;
    rdfs:comment """
        The operating organization, if different from the provider. This enables the representation of services
        that are provided by an organization, but operated by another organization like a subcontractor.
    """ .

:assistanceOperator	 a rdf:Property ;
    :domainIncludes :MobilityService ;
    :rangeIncludes :Organization,
        :ContactPoint ;
    rdfs:label "assistanceOperator" ;
    rdfs:comment """
        Operator of the assistance service for this facility. Helpful for people with impaired mobility.
        This enables the representation of services that are provided by an organization, but operated by
        another organization like a subcontractor.
    """ .

:facilityManagementOperator	 a rdf:Property ;
    :domainIncludes :MobilityService ;
    :rangeIncludes :Organization,
        :ContactPoint ;
    rdfs:label "facilityManagementOperator" ;
    rdfs:comment """
        Operator to be contacted to report service outages and other problems with this facility.
        This enables the representation of services that are provided by an organization, but operated by
        another organization like a subcontractor.
    """ .

:emergencyOperator a rdf:Property ;
    :domainIncludes :MobilityService ;
    :rangeIncludes :Organization,
        :ContactPoint ;
    rdfs:label "emergencyOperator" ;
    rdfs:comment """
        Operator to be contacted in case of an emergency. This enables the representation of services that
        are provided by an organization, but operated by another organization like a subcontractor.
    """ .

