@prefix : <https://schema.org/> .
@prefix todo: <https://todo/> .
@prefix rdf: <http://www.w3.org/1999/02/22-rdf-syntax-ns#> .
@prefix rdfs: <http://www.w3.org/2000/01/rdf-schema#> .

#
# This file contains information about Thing > Intangible > OperationalStatus.
#
# @see https://github.com/schemaorg/suggestions-questions-brainstorming/issues/39
#

#
# Classes
#
:OperationalStatus a rdfs:Class ;
    rdfs:subClassOf :Intangible;
    rdfs:label "OperationalStatus" ;
    rdfs:comment """
        Describes the current operational status of a [[Thing]].
    """ .

#
# Properties
#
:facility a rdf:Property ;
    :domainIncludes :OperationalStatus ;
    :rangeIncludes :Thing ;
    rdfs:label "facility" ;
    rdfs:comment """
        Reference to the facility that has the status described by this resource.
    """ .

:isWorking a rdf:Property ;
    :domainIncludes :OperationalStatus ;
    :rangeIncludes :Boolean ;
    rdfs:label "isWorking" ;
    rdfs:comment """
        Allows live status update. True if the equipment is currently usable, False if it's out of service.
    """ .

:timestamp a rdf:Property ;
    :domainIncludes :OperationalStatus ;
    :rangeIncludes :Date ;
    rdfs:label "timestamp" ;
    rdfs:comment """
        Describes when the live status of this equipment was last determined. Important to determine if a
        status information is outdated.
    """ .

:sources a rdf:Property ;
    :domainIncludes :OperationalStatus ;
    :rangeIncludes :URL ;
    rdfs:label "sources" ;
    rdfs:comment """
        Reference to sources for this status information.
    """ .

:alternatives a rdf:Property ;
    :domainIncludes :OperationalStatus ;
    :rangeIncludes :HowTo ;
    rdfs:label "alternatives" ;
    rdfs:comment """
        One or more HowTos that describe alternative ways a user can take when they canâ€™t use the facility
        (for excample because it is out of order).
    """ .

:outOfOrderReason a rdf:Property ;
    :domainIncludes :OperationalStatus ;
    :rangeIncludes :Text ;
    rdfs:label "outOfOrderReason" ;
    rdfs:comment """
        If the equipment is out of order, this contains a description that can provide more information
        about causes of and workarounds for the current outage (e.g. 'in maintenance until December 20, 2025.
        Please use the east entrance instead.)
    """ .

:currentVerticalDirection a rdf:Property ;
    :domainIncludes :OperationalStatus ;
    :rangeIncludes :verticalDirection ;
    rdfs:label "currentVerticalDirection" ;
    rdfs:comment """
        Current vertical direction ('up' or 'down'). Can be used to provide real-time updates, e.g. for
        Elevator or Escalator.
    """ .

