
#
# Properties
#
:count a rdf:Property ;
    :domainIncludes :ParkingFacility ;
    :rangeIncludes :QuantitativeValue ;
    rdfs:label "count" ;
    rdfs:comment """
        Defines many wheelchair accessible parking lots are provided
    """ .

:distanceToEntrance a rdf:Property ;
    :domainIncludes :ParkingFacility ;
    :rangeIncludes :QuantitativeValue ;
    rdfs:label "distanceToEntrance" ;
    rdfs:comment """
        How far away is the parking from the main entrance? If there is a separate wheelchair entrance, the
        distance to this entrance MUST be used.
    """ .

:hasDedicatedSignage a rdf:Property ;
    :domainIncludes :ParkingFacility ;
    :rangeIncludes :Boolean ;
    rdfs:label "hasDedicatedSignage" ;
    rdfs:comment """
        True if there is dedicated signage at all relevant turning points from the street to the parking,
        false if not, undefined if this is unknown.
    """ .

:isLocatedInside a rdf:Property ;
    :domainIncludes :ParkingFacility ;
    :rangeIncludes :Boolean ;
    rdfs:label "isLocatedInside" ;
    rdfs:comment """
        True if the parking is inside a building or under a roof, false if not, undefined if unknown.
    """ .

:length a rdf:Property ;
    :domainIncludes :ParkingFacility ;
    :rangeIncludes :QuantitativeValue ;
    rdfs:label "length" ;
    rdfs:comment """
        Length constraint of the parking lots.
    """ .

:location a rdf:Property ;
    :domainIncludes :ParkingFacility ;
    :rangeIncludes :Text ;
    rdfs:label "location" ;
    rdfs:comment """
        Describes where the parking is located.
    """ .

:maxVehicleHeight a rdf:Property ;
    :domainIncludes :ParkingFacility ;
    :rangeIncludes :QuantitativeValue ;
    rdfs:label "maxVehicleHeight" ;
    rdfs:comment """
        Maximal allowed vehicle height for users of this parking.
    """ .

:neededParkingPermits a rdf:Property ;
    :domainIncludes :ParkingFacility ;
    :rangeIncludes :Text ;
    rdfs:label "neededParkingPermits" ;
    rdfs:comment """
        List of permit names that allow using this parking.
    """ .

:paymentBySpace a rdf:Property ;
    :domainIncludes :ParkingFacility ;
    :rangeIncludes :Boolean ;
    rdfs:label "paymentBySpace" ;
    rdfs:comment """
        True if the parking has to be paid by space, false if not, undefined if unknown.
    """ .

:paymentByZone a rdf:Property ;
    :domainIncludes :ParkingFacility ;
    :rangeIncludes :Boolean ;
    rdfs:label "paymentByZone" ;
    rdfs:comment """
        True if the parking has to be paid by parking zone, false if not, undefined if unknown.
    """ .

:width a rdf:Property ;
    :domainIncludes :ParkingFacility ;
    :rangeIncludes :QuantitativeValue ;
    rdfs:label "width" ;
    rdfs:comment """
        Width constraint of the parking lots.
    """ .

