@prefix : <https://schema.org/> .
@prefix todo: <https://todo/> .
@prefix rdf: <http://www.w3.org/1999/02/22-rdf-syntax-ns#> .
@prefix rdfs: <http://www.w3.org/2000/01/rdf-schema#> .

#
# This file contains information about Thing > Place.
#
# @see https://github.com/schemaorg/suggestions-questions-brainstorming/issues/39
#

#
# Properties
#
:hasEntrance a rdf:Property ;
    :domainIncludes :Place ;
    :rangeIncludes :Portal ;
    rdfs:label "hasEntrances" ;
    rdfs:comment """
        Describes the entrance(s) and exit(s) from/to this place.
    """ .

:hasGroundSurface a rdf:Property ;
    :domainIncludes :Place ;
    :rangeIncludes :GroundSurface ;
    rdfs:label "hasGroundSurface" ;
    rdfs:comment """
        Describes the ground surface at this place.
        This is relevant for vehicle mobility and accessibility for people with mobility impairments.
    """ .

:hasVisitorAnimalPolicy a rdf:Property ;
    :domainIncludes :Place ;
    :rangeIncludes :AnimalPolicy ;
    rdfs:label "hasVisitorAnimalPolicy" ;
    rdfs:comment """
        Describes how the operators of this place deal with visitors accompanied by animals.
        This is relevant for people who need an assistance animal (e.g. a guide dog), or travel with a pet.
    """ .

:turningSpaceInside a rdf:Property ;
    :domainIncludes :Place ;
    :rangeIncludes :QuantitativeValue ;
    rdfs:label "turningSpaceInside" ;
    rdfs:comment """
        Describes how wide is the space inside that is usable for turning.
        If given, the value SHOULD have a minValue property.
        This is relevant for wheelchair accessibility, especially for users of electric wheelchairs.
    """ .

