@prefix : <https://schema.org/> .
@prefix todo: <https://todo/> .
@prefix rdf: <http://www.w3.org/1999/02/22-rdf-syntax-ns#> .
@prefix rdfs: <http://www.w3.org/2000/01/rdf-schema#> .

#
# This file contains information about Place > Portal.
#
# @see https://github.com/schemaorg/suggestions-questions-brainstorming/issues/39

#
# Classes
#
:Portal a rdfs:Class ;
    rdfs:subClassOf :Place;
    rdfs:label "Portal" ;
    :sameAs <https://www.wikidata.org/wiki/Q854429> ;
    rdfs:comment """
        Describes a physical entrance to a [[Place]].
        If a [[Thing]] is used as an entrance or exit, this type can be combined as multi-type entity with other types like [[Door]], [[Elevator]], [[Escalator]], or [[Ramp]].
        An [[PortalisMainPortal]] SHOULD have a name property with the name of the entrance if there are multiple entrances to the same place.
        If one or more physical sign(s) exist for the entrance, the value of name SHOULD correspond to what is readable on the sign(s).
    """ .

#
# Properties
#
:isMainPortal a rdf:Property ;
    :domainIncludes :Portal ;
    :rangeIncludes :Boolean ;
    rdfs:label "isMainPortal" ;
    rdfs:comment """
        True if this is the designated main entrance/exit for the associated place, False if not.
    """ .

:isEntrance a rdf:Property ;
    :domainIncludes :Portal ;
    :rangeIncludes :Boolean ;
    rdfs:label "isEntrance" ;
    rdfs:comment """
        True if this resource can be used by visitors to enter the Place it is contained in, False if not.
    """ .

:isExit a rdf:Property ;
    :domainIncludes :Portal ;
    :rangeIncludes :Boolean ;
    rdfs:label "isExit" ;
    rdfs:comment """
        True if this resource can be used by visitors to exit the Place it is contained in, False if not.
    """ .

:origin a rdf:Property ;
    :domainIncludes :Portal ;
    :rangeIncludes :Place, :Thing ;
    rdfs:label "origin" ;
    rdfs:comment """
        The Place or Thing from which this Portal leads to somewhere else. Use together with the
        isUnidirectional property.
    """ .

:destination a rdf:Property ;
    :domainIncludes :Portal ;
    :rangeIncludes :Place, :Thing ;
    rdfs:label "destination" ;
    rdfs:comment """
        The Place or Thing to which this Portal leads. Use together with the isUnidirectional property.
    """ .

:isUnidirectional a rdf:Property ;
    :domainIncludes :Portal ;
    :rangeIncludes :Boolean ;
    rdfs:label "isUnidirectional" ;
    rdfs:comment """
        True if users can only traverse this resource in one direction, False if it can by explicitly used
        bidirectionally. If set to True, the order of origin and destination describes the allowed traversal
        direction.
    """ .

:groundSurface a rdf:Property ;
    :domainIncludes :Portal ;
    :rangeIncludes :GroundSurface ;
    rdfs:label "groundSurface" ;
    rdfs:comment """
        Describes the ground surface traversed when using this entrance or exit. If different surfaces exist,
        this should describe the worst one for accessibility.
    """ .

:operationalStatus a rdf:Property ;
    :domainIncludes :Portal ;
    :rangeIncludes :OperationalStatus ;
    rdfs:label "operationalStatus" ;
    rdfs:comment """
        Describes current usability of the entrance/exit. Can be used for real-time status updates.
    """ .

