@prefix : <https://schema.org/> .
@prefix todo: <https://todo/> .
@prefix rdf: <http://www.w3.org/1999/02/22-rdf-syntax-ns#> .
@prefix rdfs: <http://www.w3.org/2000/01/rdf-schema#> .

#
# This file contains information about Thing > Product > Ramp.
#
# @see https://github.com/schemaorg/suggestions-questions-brainstorming/issues/39
#

#
# Classes
#
:Ramp a rdfs:Class ;
    rdfs:subClassOf :Product;
    rdfs:label "Ramp" ;
    :sameAs <https://dbpedia.org/page/Inclined_plane> ;
    :sameAs <https://www.wikidata.org/wiki/Q661343> ;
    rdfs:comment """
        A wheelchair ramp can be permanent, semi-permanent or portable. Permanent ramps are designed to be
        bolted or otherwise attached in place. Semi-permanent ramps rest on top of the ground or concrete pad
        and are commonly used for the short term. Permanent and semi-permanent ramps are usually of aluminum,
        concrete or wood. Portable ramps are usually aluminum and typically fold for ease of transport. Portable
        ramps are primarily intended for home and building use but can also be used with vans to load an
        unoccupied mobility device or to load an occupied mobility device when both the device and the passenger
        are easy to handle.
    """ .

#
# Properties
#
:isMobile a rdf:Property ;
    :domainIncludes :Ramp ;
    :rangeIncludes :Boolean ;
    rdfs:label "isMobile" ;
    rdfs:comment """
        True if the ramp is removable or mobile, False if it is fixed. Many places have smaller steps at the
        entrance, but provide a mobile ramp to compensate this when asked. This ramp is usually installed when
        a visitor calls for assistance in advance, uses a designated doorbell, or when they are seen from the
        inside.
    """ .

:incline a rdf:Property ;
    :domainIncludes :Ramp ;
    :rangeIncludes :QuantitativeValue ;
    rdfs:label "incline" ;
    rdfs:comment """
        Grade as calculated by rise / run or the tangent of the angle of inclination (e.g. '20%'), or given
        as angle of the inclination (e.g. '11.3 degrees'). See Wikipedia for a definition.
    """ .

:connectedFloorLevels a rdf:Property ;
    :domainIncludes :Ramp ;
    :rangeIncludes :Text ;
    rdfs:label "connectedFloorLevels" ;
    rdfs:comment """
        The connected floor levels in a multi-storey building, as list, if applicable. Since counting systems
        vary internationally, the local system should be used where possible.
    """ .

:operationalStatus a rdf:Property ;
    :domainIncludes :Ramp ;
    :rangeIncludes :OperationalStatus ;
    rdfs:label "operationalStatus" ;
    rdfs:comment """
        Describes current usability of the ramp. Can be used for real-time status updates.
    """ .

