@prefix : <https://schema.org/> .
@prefix todo: <https://todo/> .
@prefix rdf: <http://www.w3.org/1999/02/22-rdf-syntax-ns#> .
@prefix rdfs: <http://www.w3.org/2000/01/rdf-schema#> .

#
# This file contains information about Product > Shower.
#
# @see https://github.com/schemaorg/suggestions-questions-brainstorming/issues/40
#

#
# Classes
#
:Shower a rdfs:Class ;
    rdfs:subClassOf :Product;
    rdfs:label "Shower" ;
    :sameAs <https://dbpedia.org/page/Shower> ;
    :sameAs <https://www.wikidata.org/wiki/Q7863> ;
    rdfs:comment """
        A shower is a place in which a person bathes under a spray of typically warm
        or hot water. Indoors, there is a drain in the floor. Most showers have
        temperature, spray pressure and adjustable showerhead nozzle. The simplest
        showers have a swivelling nozzle aiming down on the user, while more complex
        showers have a showerhead connected to a hose that has a mounting bracket.
        This allows the showerer to hold the showerhead by hand to spray the water at
        different parts of their body. A shower can be installed in a small shower stall
        or bathtub with a plastic shower curtain or door.
    """ .

#
# Properties
#
:hasShowerSeat a rdf:Property ;
    :domainIncludes :Shower ;
    :rangeIncludes :Boolean ;
    rdfs:label "hasShowerSeat" ;
    rdfs:comment """
        True if the shower has a seat, False if not.
    """ .

:showerSeatIsFoldable a rdf:Property ;
    :domainIncludes :Shower ;
    :rangeIncludes :Boolean ;
    rdfs:label "showerSeatIsFoldable" ;
    rdfs:comment """
        True if the shower seat can be folded, False if not.
    """ .

:showerSeatIsRemovable a rdf:Property ;
    :domainIncludes :Shower ;
    :rangeIncludes :Boolean ;
    rdfs:label "showerSeatIsRemovable" ;
    rdfs:comment """
        True if the shower seat can be removed from the shower easily, False if not.
    """ .

:hasInShowerGrabBar a rdf:Property ;
    :domainIncludes :Shower ;
    :rangeIncludes :GrabBar ;
    rdfs:label "hasInShowerGrabBar" ;
    rdfs:comment """
        Describes grab bar that you can use to get into the shower.
    """ .

:hasIntoShowerGrabBar a rdf:Property ;
    :domainIncludes :Shower ;
    :rangeIncludes :GrabBar ;
    rdfs:label "hasIntoShowerGrabBar" ;
    rdfs:comment """
        Describes grab bar while using the shower.
    """ .

:hasTransferSeat a rdf:Property ;
    :domainIncludes :Shower ;
    :rangeIncludes :Boolean ;
    rdfs:label "hasTransferSeat" ;
    rdfs:comment """
        True if the shower has a transfer seat, false if there is no transfer seat.
    """ .
