@prefix : <https://schema.org/> .
@prefix todo: <https://todo/> .
@prefix rdf: <http://www.w3.org/1999/02/22-rdf-syntax-ns#> .
@prefix rdfs: <http://www.w3.org/2000/01/rdf-schema#> .

#
# This file contains information about Thing > Product > Stairs.
#
# @see https://github.com/schemaorg/suggestions-questions-brainstorming/issues/39
#

#
# Classes
#
:Stairs a rdfs:Class ;
    rdfs:subClassOf :Product;
    rdfs:label "Stairs" ;
    :sameAs <https://dbpedia.org/page/Stairs> ;
    :sameAs <https://www.wikidata.org/wiki/Q12511> ;
    rdfs:comment """
        A stairway, staircase, stairwell, flight of stairs, or simply stairs, is a construction designed to
        bridge a large vertical distance by dividing it into smaller vertical distances, called steps.
        Stairs may be straight, round, or may consist of two or more straight pieces connected at angles.
        Special types of stairs include escalators and ladders. Some alternatives to stairs are elevators
        (also called lifts), stairlifts and inclined moving walkways.
    """ .

#
# Properties
#
:stepHeight a rdf:Property ;
    :domainIncludes :Stairs ;
    :rangeIncludes :QuantitativeValue ;
    rdfs:label "stepHeight" ;
    rdfs:comment """
        Indicates how high the steps if these stairs are (can be a range).
    """ .

:hasAntiSlipNosing a rdf:Property ;
    :domainIncludes :Stairs ;
    :rangeIncludes :Boolean ;
    rdfs:label "hasAntiSlipNosing" ;
    rdfs:comment """
        True if all relevant steps are coated with anti-slip material, False if not.
    """ .

:hasHighContrastNosing a rdf:Property ;
    :domainIncludes :Stairs ;
    :rangeIncludes :Boolean ;
    rdfs:label "hasHighContrastNosing" ;
    rdfs:comment """
        True if all relevant steps have a visually recognizable high contrast nosing, False if not.
    """ .

:connectedFloorLevels a rdf:Property ;
    :domainIncludes :Stairs ;
    :rangeIncludes :Text ;
    rdfs:label "connectedFloorLevels" ;
    rdfs:comment """
        The connected floor levels in a multi-storey building, as list, if applicable. Since counting systems
        vary internationally, the local system should be used where possible.
    """ .

:operationalStatus a rdf:Property ;
    :domainIncludes :Stairs ;
    :rangeIncludes :OperationalStatus ;
    rdfs:label "operationalStatus" ;
    rdfs:comment """
        Describes current usability of the stairs. Can be used for real-time status updates.
    """ .

:incline a rdf:Property ;
    :domainIncludes :Stairs ;
    :rangeIncludes :QuantitativeValue ;
    rdfs:label "incline" ;
    rdfs:comment """
        Grade as calculated by rise / run or the tangent of the angle of inclination (e.g. '20%'), or given
        as angle of the inclination (e.g. '11.3 degrees'). See Wikipedia for a definition.
    """ .

