@prefix : <https://schema.org/> .
@prefix todo: <https://todo/> .
@prefix rdf: <http://www.w3.org/1999/02/22-rdf-syntax-ns#> .
@prefix rdfs: <http://www.w3.org/2000/01/rdf-schema#> .

#
# This file contains :Thing extensions.
#
# @see https://github.com/schemaorg/suggestions-questions-brainstorming/issues/41
#
:accessMode
    :domainIncludes :Thing ;
    rdfs:comment """
        a11y: This property now applies to schema:Thing instead of only schema:CreativeWork.
    """ ;
    todo:item "add :source" .

:accessModeSufficient
    :domainIncludes :Thing ;
    rdfs:comment "a11y: This property now applies to schema:Thing instead of only schema:CreativeWork." ;
    todo:item "add :source" .

:accessibilityHumanInterface a rdf:Property ;
    rdfs:label "accessibilityHumanInterface" ;
    :domainIncludes :Thing ;
    :rangeIncludes :Text ;
    rdfs:comment """
        Indicates that the resource is compatible with the referenced standardized human interface.
    """ ;
    todo:item "extend rdfs:comment, for example ISO-12345" ;
    todo:item "add :source" .

:accessibilitySummary
    :domainIncludes :Thing ;
    rdfs:comment "a11y: Properties domain now applies to schema:Thing instead of only schema:CreativeWork." ;
    todo:item "add :source" .

:physicalAccessibilityControl a rdf:Property ;
    rdfs:label "physicalAccessibilityControl" ;
    :domainIncludes :Thing ;
    :rangeIncludes :Thing ;
    todo:item "add :source" ;
    todo:item "write rdfs:comment" .

:physicalAccessibilityFeature a rdf:Property ;
    rdfs:label "physicalAccessibilityFeature" ;
    :domainIncludes :Thing ;
    :rangeIncludes :Thing ;
    todo:item "add :source" ;
    todo:item "write rdfs:comment" .

:physicalAccessibilityHazard a rdf:Property ;
    rdfs:label "physicalAccessibilityHazard" ;
    :domainIncludes :Thing ;
    :rangeIncludes :Thing ;
    todo:item "add :source" ;
    todo:item "write rdfs:comment" .
