@prefix : <https://schema.org/> .
@prefix todo: <https://todo/> .
@prefix rdf: <http://www.w3.org/1999/02/22-rdf-syntax-ns#> .
@prefix rdfs: <http://www.w3.org/2000/01/rdf-schema#> .

#
# This file contains information about Thing > Toilet.
#
# @see https://github.com/schemaorg/suggestions-questions-brainstorming/issues/40
#

#
# Classes
#
:Toilet a rdfs:Class ;
    rdfs:subClassOf :Product;
    rdfs:label "Toilet" ;
    :sameAs <https://www.wikidata.org/wiki/Q7857> ;
    rdfs:comment """
        Toilet describes the fixtures in a toilet room itself
        ([Wikipedia](https://en.wikipedia.org/wiki/Toilet)).
        Can be combined with [[Place]] to describe that it is inside a [[Room]] or [[PublicToilet]] as [[partOf]], for example.
        Note that a [[PublicToilet]] can contain multiple [[Toilet]]s.
    """ .

:SquatToilet a rdfs:Class ;
    rdfs:subClassOf :Toilet;
    rdfs:label "Squat Toilet" ;
    :sameAs <https://www.wikidata.org/wiki/Q1363734> ;
    rdfs:comment """
        A more specific type of [[Toilet]] for used by squatting.
    """ .

:Urinal a rdfs:Class ;
    rdfs:subClassOf :Toilet;
    rdfs:label "Urinal" ;
    :sameAs <https://www.wikidata.org/wiki/Q152285> ;
    rdfs:comment """
        A more specific type of [[Toilet]] for standing use and a device in which to urinate while standing ([Wikidata](https://www.wikidata.org/wiki/Q152285)).
    """ .

#
# Properties
#

:spaceOnUsersLeftSide a rdf:Property ;
    :domainIncludes :Toilet ;
    :rangeIncludes :QuantitativeValue ;
    rdfs:label "spaceOnUsersLeftSide" ;
    rdfs:comment """
        Denotes how much space is on the left side of the user (from their perspective while use).
        This is relevant for accessibility.
    """ .
