@prefix : <https://schema.org/> .
@prefix todo: <https://todo/> .
@prefix rdf: <http://www.w3.org/1999/02/22-rdf-syntax-ns#> .
@prefix rdfs: <http://www.w3.org/2000/01/rdf-schema#> .

#
# This file contains information about Thing > Toilet.
#
# @see https://github.com/schemaorg/suggestions-questions-brainstorming/issues/40
#

#
# Classes
#
:Toilet a rdfs:Class ;
    rdfs:subClassOf :Product;
    rdfs:label "Toilet" ;
    :sameAs <http://live.dbpedia.org/page/Toilet> ;
    :sameAs <https://www.wikidata.org/wiki/Q7857> ;
    rdfs:comment """
        Toilet describes the fixtures in a toilet room itself
        ([Wikipedia](https://en.wikipedia.org/wiki/Toilet)).
        Can be combined with [[Place]] to describe that it is inside a [[Room]] or [[PublicToilet]] as [[partOf]], for example.
        Note that a [[PublicToilet]] can contain multiple [[Toilet]]s.
    """ .

:SquatToilet a rdfs:Class ;
    rdfs:subClassOf :Toilet;
    rdfs:label "Squat Toilet" ;
    :sameAs <http://live.dbpedia.org/page/Squat_toilet> ;
    :sameAs <https://www.wikidata.org/wiki/Q1363734> ;
    rdfs:comment """
        A more specific type of [[Toilet]] for used by squatting.
    """ .

:Urinal a rdfs:Class ;
    rdfs:subClassOf :Toilet;
    rdfs:label "Urinal" ;
    :sameAs <http://live.dbpedia.org/page/Urinal> ;
    :sameAs <https://www.wikidata.org/wiki/Q152285> ;
    rdfs:comment """
        A more specific type of [[Toilet]] for standing use and a device in which to urinate while
        standing ([Wikidata](https://www.wikidata.org/wiki/Q152285)).
    """ .

:SeatedToilet a rdfs:Class ;
    rdfs:subClassOf :Toilet;
    rdfs:label "SeatedToilet" ;
    :sameAs <http://live.dbpedia.org/page/Urinal> ;
    :sameAs <https://www.wikidata.org/wiki/Q152285> ;
    rdfs:comment """
        A more specific type of [[Toilet]] for standing use and a device in which to urinate while
        standing ([Wikidata](https://www.wikidata.org/wiki/Q152285)).
    """ .


#
# Properties
#
:isPortable a rdf:Property ;
    :domainIncludes :Toilet ;
    :rangeIncludes :Boolean ;
    rdfs:label "isPortable" ;
    rdfs:comment """
        Denotes a more specific type of Toilet, e.g. used on festivals and construction sites
        (see https://en.wikipedia.org/wiki/Portable_toilet).
    """ .

:hasWaterSeal a rdf:Property ;
    :domainIncludes :Toilet ;
    :rangeIncludes :Boolean ;
    rdfs:label "hasWaterSeal" ;
    rdfs:comment """
        True if the toilet has a water seal, False if not.
    """ .

:spaceOnUsersLeftSide a rdf:Property ;
    :domainIncludes :Toilet ;
    :rangeIncludes :QuantitativeValue ;
    rdfs:label "spaceOnUsersLeftSide" ;
    rdfs:comment """
        Denotes how much space is on the left side of the user (from their perspective while use).
        This is relevant for accessibility.
    """ .

:spaceOnUsersRightSide a rdf:Property ;
    :domainIncludes :Toilet ;
    :rangeIncludes :QuantitativeValue ;
    rdfs:label "spaceOnUsersRightSide" ;
    rdfs:comment """
        How much space is on the right side of the user.
        This is relevant for people with mobility impairments.
    """ .

:spaceInFront a rdf:Property ;
    :domainIncludes :Toilet ;
    :rangeIncludes :QuantitativeValue ;
    rdfs:label "spaceInFront" ;
    rdfs:comment """
        How much space is on the front of the user.
        This is relevant for people with mobility impairments.
    """ .

:usageHeight a rdf:Property ;
    :domainIncludes :Toilet ;
    :rangeIncludes :QuantitativeValue ;
    rdfs:label "usageHeight" ;
    rdfs:comment """
        Indicates the distance of the toilet bowl opening or sitting height to the floor, if applicable.
        This is relevant for people with mobility impairments.
    """ .

:hasGrabBars a rdf:Property ;
    :domainIncludes :Toilet ;
    :rangeIncludes :GrabBar ;
    rdfs:label "hasGrabBars" ;
    rdfs:comment """
        Grab Bars next to the toilet.
    """ .

:hasTransferSeat a rdf:Property ;
    :domainIncludes :Toilet ;
    :rangeIncludes :Boolean ;
    rdfs:label "hasTransferSeat" ;
    rdfs:comment """
        True if the toilet has a transfer seat, false if there is no transfer seat.
    """ .

:hasHeightAdjustableNursingCouch a rdf:Property ;
    :domainIncludes :Toilet ;
    :rangeIncludes :Boolean ;
    rdfs:label "hasHeightAdjustableNursingCouch" ;
    rdfs:comment """
        True if the toilet has a height adjustable nursing couch, false if not.
    """ .

:hasElectricCeilingHoist a rdf:Property ;
    :domainIncludes :Toilet ;
    :rangeIncludes :Boolean ;
    rdfs:label "hasElectricCeilingHoist" ;
    rdfs:comment """
        True if the toilet has a has an electric ceiling hoist, false if not.
    """ .

:hasAirtightNappyPail a rdf:Property ;
    :domainIncludes :Toilet ;
    :rangeIncludes :Boolean ;
    rdfs:label "hasAirtightNappyPail" ;
    rdfs:comment """
        True if the toilet has an airtight nappy pail, false if not.
    """ .

