@prefix : <https://schema.org/> .
@prefix todo: <https://todo/> .
@prefix rdf: <http://www.w3.org/1999/02/22-rdf-syntax-ns#> .
@prefix rdfs: <http://www.w3.org/2000/01/rdf-schema#> .

#
# This file contains information about Product > WashBasin.
#
# @see https://github.com/schemaorg/suggestions-questions-brainstorming/issues/40
#

#
# Classes
#
:WashBasin a rdfs:Class ;
    rdfs:subClassOf :Product;
    rdfs:label "WashBasin" ;
    :sameAs <https://dbpedia.org/page/Sink> ;
    :sameAs <https://www.wikidata.org/wiki/Q140565> ;
    rdfs:comment """
        A sink — also known by other names including sinker, washbowl, hand basin,
        and wash basin—is a bowl-shaped plumbing fixture used for washing hands,
        dishwashing, and other purposes. Sinks have taps (faucets) that supply hot and
        cold water and may include a spray feature to be used for faster rinsing.
        They also include a drain to remove used water; this drain may itself include a
        strainer and/or shut-off device and an overflow-prevention device.
        Sinks may also have an integrated soap dispenser.
    """ .

#
# Properties
#
:topHeight a rdf:Property ;
    :domainIncludes :WashBasin ;
    :rangeIncludes :QuantitativeValue ;
    rdfs:label "topHeight" ;
    rdfs:comment """
        Defines at which height is the wash basin's top
    """ .

:bottomClearance a rdf:Property ;
    :domainIncludes :WashBasin ;
    :rangeIncludes :QuantitativeValue ;
    rdfs:label "bottomClearance" ;
    rdfs:comment """
        How high is the space below the basin? This is relevant for
        people using a wheelchair.
    """ .

:hasTransferSeat a rdf:Property ;
    :domainIncludes :WashBasin ;
    :rangeIncludes :Boolean ;
    rdfs:label "hasTransferSeat" ;
    rdfs:comment """
        True if the wash basin has a transfer seat, false if there is no transfer seat.
    """ .

:heightAdjustable a rdf:Property ;
    :domainIncludes :WashBasin ;
    :rangeIncludes :Boolean ;
    rdfs:label "heightAdjustable" ;
    rdfs:comment """
        True if the wash basin is height adjustable, false if not.
    """ .
